Types.v
@@ -32,27 +32,15 @@ Delimit Scope fieldspec_scope with fieldspec.
 
 Inductive sign : Type := plus | minus.
 
-Module Type Word.
-  (* Number of bits per byte *)
-  Context (byteWidth : {n : nat | n > 0}).
-  
-  (* Number of bytes per word *)
-  Context (wordWidth : {n : nat | n > 0}).
-  
-  Context (word : Type).
-  Context (signedFromWord : word -> Z).
-  Context (unsignedFromWord : word -> Z).
-  Context (fieldFromWord : word -> fieldspec -> Z).
-  Context (wordFromZ : Z -> word).
-End Word.
-
 Ltac easy_subset n :=
   refine (exist _ n _); try omega; auto.
 
-Module MixWord : Word.
-  (* We stay faithful to Knuth with 6-bit bytes and 5-byte words. *)
-  Definition byteWidth : {n : nat | n > 0}. easy_subset 6. Defined.
-  Definition wordWidth : {n : nat | n > 0}. easy_subset 5. Defined.
+Definition _word : {n : nat | n > 0} -> {n : nat | n > 0} -> Type := fun _ _ => Z.
+
+Section withWidth.
+  (* Parameterize operations on words over number of bits per byte and number of bytes per word. We will stay faithful to Knuth with 6-bit bytes and 5-byte words. *)
+  Context (byteWidth : {n : nat | n > 0}).
+  Context (wordWidth : {n : nat | n > 0}).
   Let byteWrap := let (bw, _) := byteWidth in
                   (2 ^ (Z.of_nat bw))%Z.
   Let wordWrap := let (bw,_) := byteWidth in
@@ -60,22 +48,23 @@ Module MixWord : Word.
               let (b,w) := (Z.of_nat bw, Z.of_nat ww) in
               (2 ^ (b*w))%Z.
 
-  Definition word : Type := Z.
+  Open Scope Z_scope.
+  Definition word : Type := _word byteWidth wordWidth.
   (* Overflow doesn't change sign. Actually, Knuth is kind of vague
   about the semantics of overflow in TAOCP, I suppose leaving it as
   undefined behavior. *)
-  Definition signedFromWord (w : word) : Z :=
+  Let signed (w : word) : Z :=
     match w with
     | Z0 => w
-    | Zpos x => (w mod wordWrap)%Z
-    | Zneg x => (- ((Zpos x) mod wordWrap))%Z
+    | Zpos x => w mod wordWrap
+    | Zneg x => - ((Zpos x) mod wordWrap)
     end.
 
-  Definition unsignedFromWord (w : word) : Z :=
+  Let unsigned (w : word) : Z :=
     match w with
     | Z0 => w
-    | Zpos x => (w mod wordWrap)%Z
-    | Zneg x => ((Zpos x) mod wordWrap)%Z
+    | Zpos x => w mod wordWrap
+    | Zneg x => (Zpos x) mod wordWrap
     end.
 
   Let signOf (w : word) : sign :=
@@ -84,34 +73,34 @@ Module MixWord : Word.
       | _ => plus
     end.
 
-  Definition wordFromZ (z : Z) : word := z.
+  Definition of_Z (z : Z) : word := signed z.
 
   Let nthByte (w : word) (n : nat) : Z :=
-    let w' := unsignedFromWord w in
+    let w' := unsigned w in
     let fix do (left : word) (m : nat) :=
         match m with
-        | O => (left mod byteWrap)%Z
-        | S m' => do (left / byteWrap)%Z m'
+        | O => left mod byteWrap
+        | S m' => do (left / byteWrap) m'
         end
     in do w' n.
 
   Let bytesOf (w : word) : list Z :=
-    let w' := unsignedFromWord w in
+    let w' := unsigned w in
     let fix do (w : word) (n : nat) (acc : list Z) :=
         match n with
-        | O => (w mod byteWrap)%Z :: acc
-        | S n' => do (w / byteWrap)%Z n' ((w mod byteWrap)%Z :: acc)
+        | O => w mod byteWrap :: acc
+        | S n' => do (w / byteWrap) n' (w mod byteWrap :: acc)
         end
-    in do w' 5 [].
+    in do w' 4%nat [].
 
-  Let bytesToWord (bs : list Z) : word :=
+  Let of_bytes (bs : list Z) : word :=
     let fix do (bs : list Z) (acc : Z) (n : Z) :=
         match bs with
-        | b :: bs => do bs (acc + (b * (byteWrap ^ n)))%Z (n - 1)%Z
+        | b :: bs => do bs (acc + (b * (byteWrap ^ n))) (n - 1)
         | [] => acc
         end
     in let n := Z.of_nat(length bs) in
-       do bs 0%Z (n-1)%Z.
+       do bs 0 (n-1).
 
   Let slice {A} (l : list A) (L R : nat) : list A :=
     (* slice the list l, yielding a list containing the elements l[i] for i \in [L-1, R) *)
@@ -129,17 +118,17 @@ Module MixWord : Word.
         | [] => List.rev acc
         end
     in
-    do l (L-1) R [].
+    do l (L-1)%nat R [].
   
-  Definition fieldFromWord (w : word) (F : fieldspec) : word :=
+  Definition fieldOf (w : word) (F : fieldspec) : word :=
     let (L, R) := F in
-    match (R ?= L) with
+    match (R ?= L)%nat with
     | Gt =>
       let (s,v) := (match L with
                     (* the field includes the sign bit *)
-                    | Zero => (signOf w, unsignedFromWord w)
+                    | Zero => (signOf w, unsigned w)
                     (* the field includes'nt the sign bit *)
-                    | otherwise => (plus, unsignedFromWord w)
+                    | otherwise => (plus, unsigned w)
                     end) in
       (* Grab bytes L through R from the word w and treats them as a
          word of their own with sign s, where the rightmost byte of the
@@ -147,138 +136,23 @@ Module MixWord : Word.
          word *)
       let bs := bytesOf w in
       let fieldSlice := slice bs L (R + 1) in
-      let newWord := (unsignedFromWord (bytesToWord fieldSlice)) in 
+      let newWord := (unsigned (of_bytes fieldSlice)) in 
       match s with
       | plus => newWord
       | minus => (- newWord)%Z
       end
     | otherwise => 0%Z (* when requesting a field of width 0 or less, just return the trivial word. *)
     end.
-End MixWord.
+End withWidth.
 
-Compute MixWord.unsignedFromWord (MixWord.wordFromZ  50%Z).
+Definition _6 : {n : nat | n > 0}. easy_subset 6. Defined.
+Definition _5 : {n : nat | n > 0}. easy_subset 5. Defined.
+Definition _2 : {n : nat | n > 0}. easy_subset 2. Defined.
+Notation word5 := (word _6 _5).
+Notation word2 := (word _6 _2).
 
-Module Type Short.
-  (* Number of bits per byte *)
-  Context (byteWidth : {n : nat | n > 0}).
-  
-  (* Number of bytes per short *)
-  Context (shortWidth : {n : nat | n > 0}).
-  
-  Context (short : Type).
-  Context (signedFromShort : short -> Z).
-  Context (unsignedFromShort : short -> Z).
-  Context (fieldFromShort : short -> fieldspec -> Z).
-  Context (shortFromZ : Z -> short).
-End Short.
+Definition of_Z5 : Z -> word5 := of_Z _6 _5.
+Definition of_Z2 : Z -> word2 := of_Z _6 _2.
 
-Delimit Scope fieldspec_scope with F.
-Import MixWord.
-Goal 50%Z = (MixWord.fieldFromWord (MixWord.wordFromZ 50) (0%F ,5%F)).
-
-
-Module MixShort : Short.
-  (* We stay faithful to Knuth with 6-bit bytes and 5-byte words. *)
-  Definition byteWidth : {n : nat | n > 0}. easy_subset 6. Defined.
-  Definition shortWidth : {n : nat | n > 0}. easy_subset 2. Defined.
-  Let byteWrap := let (bw, _) := byteWidth in
-                  (2 ^ (Z.of_nat bw))%Z.
-  Let shortWrap := let (bw,_) := byteWidth in
-              let (ww,_) := shortWidth in
-              let (b,w) := (Z.of_nat bw, Z.of_nat ww) in
-              (2 ^ (b*w))%Z.
-
-  Definition short : Type := Z.
-  (* Overflow doesn't change sign. Actually, Knuth is kind of vague
-  about the semantics of overflow in TAOCP, I suppose leaving it as
-  undefined behavior. *)
-  Definition signedFromShort (s : short) : Z :=
-    match s with
-    | Z0 => s
-    | Zpos x => (s mod shortWrap)%Z
-    | Zneg x => (- ((Zpos x) mod shortWrap))%Z
-    end.
-
-  Definition unsignedFromWord (w : word) : Z :=
-    match w with
-    | Z0 => w
-    | Zpos x => (w mod wordWrap)%Z
-    | Zneg x => ((Zpos x) mod wordWrap)%Z
-    end.
-
-  Let signOf (w : word) : sign :=
-    match w with
-      | Zneg _ => minus
-      | _ => plus
-    end.
-
-  Definition wordFromZ (z : Z) : word := z.
-
-  Let nthByte (w : word) (n : nat) : Z :=
-    let w' := unsignedFromWord w in
-    let fix do (left : word) (m : nat) :=
-        match m with
-        | O => (left mod byteWrap)%Z
-        | S m' => do (left / byteWrap)%Z m'
-        end
-    in do w' n.
-
-  Let bytesOf (w : word) : list Z :=
-    let w' := unsignedFromWord w in
-    let fix do (w : word) (n : nat) (acc : list Z) :=
-        match n with
-        | O => (w mod byteWrap)%Z :: acc
-        | S n' => do (w / byteWrap)%Z n' ((w mod byteWrap)%Z :: acc)
-        end
-    in do w' 5 [].
-
-  Let bytesToWord (bs : list Z) : word :=
-    let fix do (bs : list Z) (acc : Z) (n : Z) :=
-        match bs with
-        | b :: bs => do bs (acc + (b * (byteWrap ^ n)))%Z (n - 1)%Z
-        | [] => acc
-        end
-    in let n := Z.of_nat(length bs) in
-       do bs 0%Z (n-1)%Z.
-
-  Let slice {A} (l : list A) (L R : nat) : list A :=
-    (* slice the list l, yielding a list containing the elements l[i] for i \in [L-1, R) *)
-    let fix do (l : list A) (L R : nat) (acc : list A) :=
-        match l with
-        | l :: ls => 
-          match L with
-          | O =>
-            match R with
-            | O => List.rev acc
-            | S R' => do ls L R' (l :: acc)
-            end
-          | S L' => do ls L' R acc
-          end
-        | [] => List.rev acc
-        end
-    in
-    do l (L-1) R [].
-  
-  Definition fieldFromWord (w : word) (F : fieldspec) : word :=
-    let (L, R) := F in
-    match (R ?= L) with
-    | Gt =>
-      let (s,v) := (match L with
-                    (* the field includes the sign bit *)
-                    | Zero => (signOf w, unsignedFromWord w)
-                    (* the field includes'nt the sign bit *)
-                    | otherwise => (plus, unsignedFromWord w)
-                    end) in
-      (* Grab bytes L through R from the word w and treats them as a
-         word of their own with sign s, where the rightmost byte of the
-         selection occupying the rightmost position in the resulting
-         word *)
-      let bs := bytesOf w in
-      let fieldSlice := slice bs L (R + 1) in
-      let newWord := (unsignedFromWord (bytesToWord fieldSlice)) in 
-      match s with
-      | plus => newWord
-      | minus => (- newWord)%Z
-      end
-    | otherwise => 0%Z (* when requesting a field of width 0 or less, just return the trivial word. *)
-    end.
+Definition fieldOf5 : word5 -> fieldspec -> Z := fieldOf _6 _5.
+Definition fieldOf2 : word2 -> fieldspec -> Z := fieldOf _6 _2.
